added state_was_set_some_id

dy-extensions/DY.Extend.fst
@@ -5,6 +5,23 @@ open DY.Core
 open DY.Lib
 open DY.Core.Trace.Base
 
+let state_was_set_some_id (#a:Type) {|local_state a|} tr prin (cont : a) =
+  exists sid. DY.Lib.state_was_set tr prin sid cont
+
+val state_was_set_some_id_grows:
+  #a:Type -> {|lsa:local_state a|} ->
+  tr1:trace -> tr2:trace -> 
+  prin:principal -> content:a ->
+  Lemma
+  (requires tr1 <$ tr2
+    /\ state_was_set_some_id tr1 prin content
+  )
+  (ensures
+    state_was_set_some_id tr2 prin content
+  )
+  [SMTPat (state_was_set_some_id #a #lsa tr1 prin content); SMTPat (tr1 <$ tr2)]
+let state_was_set_some_id_grows #a #ls tr1 tr2 prin content  = admit()
+
 
 /// Lookup the most recent state of a principal satisfying some property.
 /// Returns the state and corresponding state id,
